src/HOL/SPARK/SPARK.thy
@@ -39,13 +39,7 @@ lemmas [simp] =
 lemma bit_not_spark_eq:
   "NOT (word_of_int x :: ('a::len) word) =
   word_of_int (2 ^ LENGTH('a) - 1 - x)"
-proof -
-  have "word_of_int x + NOT (word_of_int x) =
-    word_of_int x + (word_of_int (2 ^ LENGTH('a) - 1 - x)::'a word)"
-    by (simp only: bwsimps bin_add_not Min_def)
-      (simp add: word_of_int_hom_syms word_of_int_2p_len)
-  then show ?thesis by (rule add_left_imp_eq)
-qed
+  by (simp flip: mask_eq_exp_minus_1 add: of_int_mask_eq not_eq_complement)
 
 lemmas [simp] =
   bit_not_spark_eq [where 'a=8, simplified]
